Modeling how distributed system reflects trace, and proving things about movers and reduction

ironfleet/src/Dafny/Distributed/Concur/Trace.i.dfy
@@ -12,6 +12,7 @@ module TraceModule {
 
     datatype Packet = Packet(dst:EndPoint, src:EndPoint, msg:seq<byte>)
     datatype Actor = NoActor() | HostActor(ep:EndPoint) | ThreadActor(tep:EndPoint, tid:int)
+    type ActorState
 
     datatype IOAction =   IOActionReceive(r:Packet)
                         | IOActionSend(s:Packet)
@@ -19,7 +20,7 @@ module TraceModule {
                         | IOActionUpdateLocalState()
                         | IOActionStutter()
 
-    datatype DSAction =   DSActionIOs(ios:seq<IOAction>)
+    datatype DSAction =   DSActionHostEventHandler(ios:seq<IOAction>)
                         | DSActionDeliverPacket(p:Packet)
                         | DSActionAdvanceTime(t:int)
                         | DSActionStutter()
