ironfleet/src/Dafny/Distributed/Concur/DistributedSystem.i.dfy
@@ -1,0 +1,118 @@
+include "Trace.i.dfy"
+
+module DistributedSystemModule {
+
+    import opened TraceModule
+
+    datatype DistributedSystem = DistributedSystem(states:map<Actor, ActorState>, time:int, sentPackets:set<Packet>)
+
+    predicate DistributedSystemInit(ds:DistributedSystem)
+    {
+           |ds.sentPackets| == 0
+        && ds.time >= 0
+    }
+
+    predicate DistributedSystemNextDSActionHostEventHandler(
+        ds:DistributedSystem,
+        ds':DistributedSystem,
+        actor:Actor,
+        ios:seq<IOAction>
+        )
+    {
+           actor.HostActor?
+        && (forall any_actor :: any_actor !in ds.states ==> any_actor !in ds'.states)
+        && (forall other_actor :: other_actor != actor && other_actor in ds.states ==>
+                            other_actor in ds'.states && ds'.states[other_actor] == ds.states[other_actor])
+        && (actor in ds.states <==> actor in ds'.states)
+        && ds'.time == ds.time
+        && (forall p :: p in ds.sentPackets ==> p in ds'.sentPackets)
+        && (forall p :: p in ds'.sentPackets ==> p in ds.sentPackets || IOActionSend(p) in ios)
+        && (forall io :: io in ios && io.IOActionReceive? ==> io.r in ds.sentPackets && io.r.dst == actor.ep)
+        && (forall io :: io in ios && io.IOActionSend? ==> io.s in ds'.sentPackets && io.s.src == actor.ep)
+    }
+
+    predicate DistributedSystemNextDSActionAdvanceTime(ds:DistributedSystem, ds':DistributedSystem, t:int)
+    {
+           t > ds.time
+        && ds' == ds.(time := t)
+    }
+
+    predicate DistributedSystemNextDSActionDeliverPacket(ds:DistributedSystem, ds':DistributedSystem, p:Packet)
+    {
+           p in ds.sentPackets
+        && ds' == ds
+    }
+
+    predicate DistributedSystemNextStutter(ds:DistributedSystem, ds':DistributedSystem)
+    {
+        ds' == ds
+    }
+
+    predicate DistributedSystemNextDSAction(ds:DistributedSystem, ds':DistributedSystem, actor:Actor, action:DSAction)
+    {
+        match action
+            case DSActionHostEventHandler(ios) => DistributedSystemNextDSActionHostEventHandler(ds, ds', actor, ios)
+            case DSActionDeliverPacket(p) => DistributedSystemNextDSActionDeliverPacket(ds, ds', p)
+            case DSActionAdvanceTime(t) => DistributedSystemNextDSActionAdvanceTime(ds, ds', t)
+            case DSActionStutter => DistributedSystemNextStutter(ds, ds')
+    }
+
+    predicate DistributedSystemNextIOActionReceive(ds:DistributedSystem, ds':DistributedSystem, actor:Actor, p:Packet)
+    {
+           ds' == ds
+        && actor.HostActor?
+        && p in ds.sentPackets
+        && p.dst == actor.ep
+    }
+
+    predicate DistributedSystemNextIOActionSend(ds:DistributedSystem, ds':DistributedSystem, actor:Actor, p:Packet)
+    {
+           ds' == ds.(sentPackets := ds.sentPackets + {p})
+        && actor.HostActor?
+        && p.src == actor.ep
+    }
+
+    predicate DistributedSystemNextIOActionReadClock(ds:DistributedSystem, ds':DistributedSystem, actor:Actor, t:int)
+    {
+           ds' == ds
+        && actor.HostActor?
+        && t == ds.time
+    }
+
+    predicate DistributedSystemNextIOActionUpdateLocalState(ds:DistributedSystem, ds':DistributedSystem, actor:Actor)
+    {
+           actor.HostActor?
+        && (forall any_actor :: any_actor !in ds.states ==> any_actor !in ds'.states)
+        && (forall other_actor :: other_actor != actor && other_actor in ds.states ==>
+                            other_actor in ds'.states && ds'.states[other_actor] == ds.states[other_actor])
+        && (actor in ds.states <==> actor in ds'.states)
+        && ds'.sentPackets == ds.sentPackets
+        && ds'.time == ds.time
+    }
+
+    predicate DistributedSystemNextIOAction(ds:DistributedSystem, ds':DistributedSystem, actor:Actor, action:IOAction)
+    {
+        match action
+            case IOActionReceive(p) => DistributedSystemNextIOActionReceive(ds, ds', actor, p)
+            case IOActionSend(p) => DistributedSystemNextIOActionSend(ds, ds', actor, p)
+            case IOActionReadClock(t) => DistributedSystemNextIOActionReadClock(ds, ds', actor, t)
+            case IOActionUpdateLocalState => DistributedSystemNextIOActionUpdateLocalState(ds, ds', actor)
+            case IOActionStutter => DistributedSystemNextStutter(ds, ds')
+    }
+
+    predicate DistributedSystemNextAction(ds:DistributedSystem, ds':DistributedSystem, actor:Actor, action:Action)
+    {
+        match action
+            case ActionIO(io_action) => DistributedSystemNextIOAction(ds, ds', actor, io_action)
+            case ActionDS(ds_action) => DistributedSystemNextDSAction(ds, ds', actor, ds_action)
+    }
+
+    predicate DistributedSystemNextEntryAction(ds:DistributedSystem, ds':DistributedSystem, entry:Entry)
+    {
+        match entry
+            case EntryAction(actor, action) => DistributedSystemNextAction(ds, ds', actor, action)
+            case EntryBeginGroup(actor, level) => DistributedSystemNextStutter(ds, ds')
+            case EntryEndGroup(actor, l1, l2, action) => DistributedSystemNextStutter(ds, ds')
+    }
+
+}
