ironfleet/src/Dafny/Distributed/Concur/EventHandler.i.dfy
@@ -1,0 +1,86 @@
+include "DistributedSystem.i.dfy"
+include "Movers.i.dfy"
+
+module EventHandlerModule {
+    import opened DistributedSystemModule
+    import opened MoversModule
+
+    function CombineIOActions(ios:seq<IOAction>) : seq<IOAction>
+    {
+        if |ios| == 0 then
+            []
+        else
+            var head_action := ios[0];
+            if head_action.IOActionUpdateLocalState? || head_action.IOActionStutter? then
+                CombineIOActions(ios[1..])
+            else
+                [head_action] + CombineIOActions(ios[1..])
+    }
+
+    function CombineIOActionsIntoDSActionHostEventHandler(ios:seq<IOAction>) : DSAction
+        ensures CombineIOActionsIntoDSActionHostEventHandler(ios).DSActionHostEventHandler?;
+    {
+        DSActionHostEventHandler(CombineIOActions(ios))
+    }
+
+    lemma lemma_CombineIOActionsPreservesNonUpdateStutters(ios:seq<IOAction>, io:IOAction)
+        requires io in ios;
+        requires !io.IOActionUpdateLocalState?;
+        requires !io.IOActionStutter?;
+        ensures  io in CombineIOActions(ios);
+    {
+    }
+
+    lemma lemma_CombineIOActionsIntroducesNoNewIOs(ios:seq<IOAction>, io:IOAction)
+        requires io in CombineIOActions(ios);
+        ensures  io in ios;
+    {
+    }
+
+    lemma lemma_EffectOfCombiningIOActionsMatchesEffectOfDoingIOActions(
+        actor:Actor,
+        io_actions:seq<IOAction>,
+        ds_action:DSAction,
+        states:seq<DistributedSystem>
+        )
+        requires actor.HostActor?;
+        requires |states| == |io_actions| + 1;
+        requires forall i :: 0 <= i < |io_actions| ==> DistributedSystemNextIOAction(states[i], states[i+1], actor, io_actions[i]);
+        requires ds_action == CombineIOActionsIntoDSActionHostEventHandler(io_actions);
+        requires IOActionsCompatibleWithReduction(io_actions);
+        ensures  DistributedSystemNextDSAction(states[0], states[|io_actions|], actor, ds_action);
+    {
+        if |io_actions| == 0 {
+            return;
+        }
+
+        var ds_action_all_but_last := CombineIOActionsIntoDSActionHostEventHandler(io_actions[1..]);
+        lemma_IfIOActionsCompatibleWithReductionThenSuffixIs(io_actions);
+        lemma_EffectOfCombiningIOActionsMatchesEffectOfDoingIOActions(actor, io_actions[1..], ds_action_all_but_last, states[1..]);
+
+        var ds := states[0];
+        var ds' := states[|io_actions|];
+        var ios := ds_action.ios;
+
+        var first_action := io_actions[0];
+
+        if first_action.IOActionSend? {
+            forall io | io in io_actions
+                ensures !io.IOActionReceive?
+            {
+                var i :| 0 <= i < |io_actions| && io_actions[i] == io;
+                if i != 0 {
+                    lemma_IfIOActionsCompatibleWithReductionAndOneIsntRightMoverThenRestAreLeftMovers(io_actions, 0, i);
+                }
+            }
+    
+            forall io | io in ios && io.IOActionReceive?
+                ensures false;
+            {
+                lemma_CombineIOActionsIntroducesNoNewIOs(io_actions, io);
+            }
+        }
+
+    }
+
+}
