ironfleet/src/Dafny/Distributed/Concur/Movers.i.dfy
@@ -1,0 +1,254 @@
+include "DistributedSystem.i.dfy"
+
+module MoversModule {
+
+    import opened DistributedSystemModule
+
+    predicate IOActionIsRightMover(io:IOAction)
+    {
+        io.IOActionReceive? || io.IOActionUpdateLocalState? || io.IOActionStutter?
+    }
+
+    predicate IOActionIsLeftMover(io:IOAction)
+    {
+        io.IOActionSend? || io.IOActionUpdateLocalState? || io.IOActionStutter?
+    }
+
+    predicate ActionIsRightMover(action:Action)
+    {
+        action.ActionIO? && IOActionIsRightMover(action.io)
+    }
+
+    predicate ActionIsLeftMover(action:Action)
+    {
+        action.ActionIO? && IOActionIsLeftMover(action.io)
+    }
+
+    predicate IOActionsCompatibleWithReductionUsingPivot(ios:seq<IOAction>, pivot:int)
+    {
+           0 <= pivot < |ios|
+        && (forall i :: 0 <= i < pivot ==> IOActionIsRightMover(ios[i]))
+        && (forall i :: pivot < i < |ios| ==> IOActionIsLeftMover(ios[i]))
+    }
+
+    predicate IOActionsCompatibleWithReduction(ios:seq<IOAction>)
+    {
+        |ios| == 0 || exists pivot :: IOActionsCompatibleWithReductionUsingPivot(ios, pivot)
+    }
+
+    lemma lemma_IfIOActionsCompatibleWithReductionAndOneIsntRightMoverThenRestAreLeftMovers(ios:seq<IOAction>, i:int, j:int)
+        requires 0 <= i < j < |ios|;
+        requires IOActionsCompatibleWithReduction(ios);
+        requires !IOActionIsRightMover(ios[i]);
+        ensures  IOActionIsLeftMover(ios[j]);
+        decreases j;
+    {
+        var pivot :| IOActionsCompatibleWithReductionUsingPivot(ios, pivot);
+        assert !(i < pivot);
+        assert j > pivot;
+    }
+
+    lemma lemma_IfIOActionsCompatibleWithReductionThenSuffixIs(ios:seq<IOAction>)
+        requires |ios| > 0;
+        requires IOActionsCompatibleWithReduction(ios);
+        ensures  IOActionsCompatibleWithReduction(ios[1..]);
+    {
+        var ios' := ios[1..];
+        if |ios'| == 0 {
+            return;
+        }
+        
+        var pivot :| IOActionsCompatibleWithReductionUsingPivot(ios, pivot);
+        if pivot == 0 {
+            assert IOActionsCompatibleWithReductionUsingPivot(ios', 0);
+        }
+        else {
+            assert IOActionsCompatibleWithReductionUsingPivot(ios', pivot-1);
+        }
+    }
+
+/*
+    lemma lemma_MoverCommutativityIO(
+        actor1:Actor,
+        actor2:Actor,
+        io1:IOAction,
+        io2:IOAction,
+        ds1:DistributedSystem,
+        ds2:DistributedSystem,
+        ds3:DistributedSystem
+        )
+        returns
+        (ds2':DistributedSystem)
+        requires actor1 != actor2;
+        requires DistributedSystemNextIOAction(ds1, ds2, actor1, io1);
+        requires DistributedSystemNextIOAction(ds2, ds3, actor2, io2);
+        requires IOActionIsRightMover(io1) || IOActionIsLeftMover(io2);
+        ensures  DistributedSystemNextIOAction(ds1, ds2', actor2, io2);
+        ensures  DistributedSystemNextIOAction(ds2', ds3, actor1, io1);
+    {
+        if io1.IOActionReceive? {
+            ds2' := ds3;
+        }
+        else if io1.IOActionUpdateLocalState? {
+            if actor1 in ds1.states {
+                ds2' := ds3.(states := ds3.states[actor1 := ds1.states[actor1]]);
+                if !io2.IOActionUpdateLocalState? {
+                    assert ds2'.states == ds1.states;
+                }
+            }
+            else {
+                assert ds1.states == ds2.states;
+                ds2' := ds3;
+            }
+        }
+        else if io1.IOActionStutter? {
+            ds2' := ds3;
+        }
+        else if io2.IOActionStutter? {
+            ds2' := ds1;
+        }
+        else if io2.IOActionUpdateLocalState? {
+            if actor2 in ds2.states {
+                ds2' := ds1.(states := ds3.states);
+            }
+            else {
+                ds2' := ds1;
+                assert ds2.states == ds3.states;
+            }
+        }
+        else if io2.IOActionSend? {
+            ds2' := ds1.(sentPackets := ds1.sentPackets + {io2.s});
+            if io1.IOActionSend? {
+                assert ds3.sentPackets == ds2'.sentPackets + {io1.s};
+            }
+        }
+    }
+
+
+    lemma lemma_MoverCommutativity(
+        actor1:Actor,
+        actor2:Actor,
+        action1:Action,
+        action2:Action,
+        ds1:DistributedSystem,
+        ds2:DistributedSystem,
+        ds3:DistributedSystem
+        )
+        returns
+        (ds2':DistributedSystem)
+        requires actor1 != actor2;
+        requires DistributedSystemNextAction(ds1, ds2, actor1, action1);
+        requires DistributedSystemNextAction(ds2, ds3, actor2, action2);
+        requires ActionIsRightMover(action1) || ActionIsLeftMover(action2);
+        ensures  DistributedSystemNextAction(ds1, ds2', actor2, action2);
+        ensures  DistributedSystemNextAction(ds2', ds3, actor1, action1);
+    {
+        if action1.ActionIO? && action2.ActionIO? {
+            ds2' := lemma_MoverCommutativityIO(actor1, actor2, action1.io, action2.io, ds1, ds2, ds3);
+            return;
+        }
+
+        if action1.ActionIO? && action1.io.IOActionReceive? {
+            ds2' := ds3;
+        }
+        else if action1.ActionIO? && action1.io.IOActionUpdateLocalState? {
+            if actor1 in ds1.states {
+                ds2' := ds3.(states := ds3.states[actor1 := ds1.states[actor1]]);
+                if !action2.ds.DSActionHostEventHandler? {
+                    assert ds2'.states == ds1.states;
+                }
+            }
+            else {
+                assert ds1.states == ds2.states;
+                ds2' := ds3;
+            }
+        }
+        else if action1.ActionIO? && action1.io.IOActionStutter? {
+            ds2' := ds3;
+        }
+        else if action2.ActionIO? && action2.io.IOActionStutter? {
+            ds2' := ds1;
+        }
+        else if action2.ActionIO? && action2.io.IOActionUpdateLocalState? {
+            if actor2 in ds2.states {
+                assume false;
+                ds2' := ds1.(states := ds3.states);
+            }
+            else {
+                ds2' := ds1;
+                assert ds2.states == ds3.states;
+            }
+        }
+        else if action2.ActionIO? && action2.io.IOActionSend? {
+            ds2' := ds1.(sentPackets := ds1.sentPackets + {action2.io.s});
+            if !action1.ds.DSActionHostEventHandler? {
+                assert ds2'.states == ds3.states;
+            }
+        }
+    }
+*/
+
+    lemma lemma_MoverCommutativity(
+        actor1:Actor,
+        actor2:Actor,
+        action1:Action,
+        action2:Action,
+        ds1:DistributedSystem,
+        ds2:DistributedSystem,
+        ds3:DistributedSystem
+        )
+        returns
+        (ds2':DistributedSystem)
+        requires actor1 != actor2;
+        requires DistributedSystemNextAction(ds1, ds2, actor1, action1);
+        requires DistributedSystemNextAction(ds2, ds3, actor2, action2);
+        requires ActionIsRightMover(action1) || ActionIsLeftMover(action2);
+        ensures  DistributedSystemNextAction(ds1, ds2', actor2, action2);
+        ensures  DistributedSystemNextAction(ds2', ds3, actor1, action1);
+    {
+        if action1.ActionIO? && action1.io.IOActionReceive? {
+            ds2' := ds3;
+        }
+        else if action1.ActionIO? && action1.io.IOActionUpdateLocalState? {
+            if actor1 in ds1.states {
+                ds2' := ds3.(states := ds3.states[actor1 := ds1.states[actor1]]);
+                if !(action2.ActionIO? && action2.io.IOActionUpdateLocalState?) &&
+                   !(action2.ActionDS? && action2.ds.DSActionHostEventHandler?) {
+                    assert ds2'.states == ds1.states;
+                }
+            }
+            else {
+                assert ds1.states == ds2.states;
+                ds2' := ds3;
+            }
+        }
+        else if action1.ActionIO? && action1.io.IOActionStutter? {
+            ds2' := ds3;
+        }
+        else if action2.ActionIO? && action2.io.IOActionStutter? {
+            ds2' := ds1;
+        }
+        else if action2.ActionIO? && action2.io.IOActionUpdateLocalState? {
+            if actor2 in ds2.states {
+                assume false;
+                ds2' := ds1.(states := ds3.states);
+            }
+            else {
+                ds2' := ds1;
+                assert ds2.states == ds3.states;
+            }
+        }
+        else if action2.ActionIO? && action2.io.IOActionSend? {
+            ds2' := ds1.(sentPackets := ds1.sentPackets + {action2.io.s});
+            if action1.ActionIO? && action1.io.IOActionSend? {
+                assert ds2'.states == ds3.states;
+                assert ds3.sentPackets == ds2'.sentPackets + {action1.io.s};
+            }
+            else if action1.ActionDS? && action1.ds.DSActionHostEventHandler? {
+                assert ds2'.states == ds1.states;
+            }
+        }
+    }
+
+}
+    
